Lamumu.lean
@@ -1,7 +1,8 @@
 -- This module serves as the root of the `Lamumu` library.
 -- Import modules here that should be built as part of the library.
 import Lamumu.Basic
+import Lamumu.Binding
 import Lamumu.Evaluator
+import Lamumu.Focusing
 import Lamumu.Notation
 import Lamumu.Pretty
-import Lamumu.Substitution
