Lamumu/Evaluator.lean
@@ -1,5 +1,6 @@
 import Lamumu.Basic
-import Lamumu.Substitution
+import Lamumu.Binding
+import Std.Tactic
 
 namespace Evaluate
 
@@ -27,8 +28,8 @@ structure EvalError where
  deriving Repr, DecidableEq
 
 def step : Statement → Except EvalError Statement
- | .cut (.mu α s) c => bif c.isCoValue then substCoVar c α s |> .ok else .error ⟨s⟩
- | .cut p (.mu_tilde x s) => if p.isValue then substVar p x s |> .ok else .error ⟨s⟩
+ | .cut (.mu _ s) c => bif c.isCoValue then openCoVarStmt 0 c s |> .ok else .error ⟨s⟩
+ | .cut p (.mu_tilde _ s) => if p.isValue then openVarStmt 0 p s |> .ok else .error ⟨s⟩
  | .prim op (.lit n) (.lit m) c => .cut (Op.eval op n m |> .lit) c |> .ok
  | .ifz (.lit 0) s1 _ => s1 |> .ok
  | .ifz _ _ s2 => s2 |> .ok
@@ -36,44 +37,3 @@ def step : Statement → Except EvalError Statement
 
 end Evaluate
 
-
-namespace Focus
-
-open Core
-
-mutual
-partial def focus (s : Statement) : Statement :=
-  match s with
-  | .cut p c => .cut (focusProducer p) (focusConsumer c)
-  | .prim op p1 p2 c =>
-    if p1.isValue && p2.isValue then
-        .prim op (focusProducer p1) (focusProducer p2) (focusConsumer c)
-    else if p1.isValue then
-        let x := freshVarFrom [freeVarsStmt s]
-        .cut (focusProducer p2)
-          (.mu_tilde x (focus (.prim op p1 (.var x) c)))
-    else
-        let x := freshVarFrom [freeVarsStmt s]
-        .cut (focusProducer p1)
-          (.mu_tilde x (focus (.prim op (.var x) p2 c)))
-  | .ifz p s1 s2 =>
-    if p.isValue then
-      .ifz (focusProducer p) (focus s1) (focus s2)
-    else
-      let x := freshVarFrom [freeVarsStmt s1, freeVarsStmt s2]
-      .cut (focusProducer p) (.mu_tilde x (.ifz x s1 s2))
-
-partial def focusProducer (p : Producer) : Producer :=
-  match p with
-  | .lit _ => p
-  | .var _ => p
-  | .mu c s => .mu c (focus s)
-
-partial def focusConsumer (c : Consumer) : Consumer :=
-  match c with
-  | .covar _ => c
-  | .mu_tilde v s => .mu_tilde v (focus s)
-
-end
-
-end Focus
