Lamumu/Pretty.lean
@@ -5,12 +5,14 @@ namespace Core
 
 open Std
 
-def ppVar (v : Var) : String :=
-  s!"x_{v}"
+def ppVar : Var → String
+  | .free n => s!"x_{n}"
+  | .bound n => s!"x_{n}"
 
 def ppCoVar : CoVar → String
   | .star => "★"
-  | .idx n => s!"α_{n}"
+  | .free n => s!"α_{n}"
+  | .bound n => s!"α_{n}"
 
 def ppOp : Op -> String
   | .add => "+"
@@ -18,20 +20,37 @@ def ppOp : Op -> String
   | .sub => "-"
 
 mutual
-  def ppProducer : Producer -> String
-    | .var v => ppVar v
+  def ppProducerCtx (vctx : List Var) (cctx : List CoVar) : Producer -> String
+    | .var v =>
+        match v with
+        | .bound i => ppVar (vctx.getD i (.free 0))
+        | .free _ => ppVar v
     | .lit n => s!"⌜{n}⌝"
-    | .mu a s => s!"μ {ppCoVar a} . {ppStatement s}"
+    | .mu a s => s!"μ {ppCoVar a} . {ppStatementCtx vctx (a :: cctx) s}"
 
-  def ppConsumer : Consumer -> String
-    | .covar a => ppCoVar a
-    | .mu_tilde a s => s!"μ̃ {ppVar a} . {ppStatement s}"
+  def ppConsumerCtx (vctx : List Var) (cctx : List CoVar) : Consumer -> String
+    | .covar a =>
+        match a with
+        | .bound i => ppCoVar (cctx.getD i (.free 0))
+        | _ => ppCoVar a
+    | .mu_tilde a s => s!"μ̃ {ppVar a} . {ppStatementCtx (a :: vctx) cctx s}"
 
-  def ppStatement : Statement -> String
-    | .prim op p1 p2 c => s!"{ppOp op}({ppProducer p1}, {ppProducer p2}; {ppConsumer c})"
-    | .ifz p s1 s2 => s!"ifz({ppProducer p}, {ppStatement s1}, {ppStatement s2})"
-    | .cut p c => s!"⟨{ppProducer p} | {ppConsumer c}⟩"
+  def ppStatementCtx (vctx : List Var) (cctx : List CoVar) : Statement -> String
+    | .prim op p1 p2 c =>
+        s!"{ppOp op}({ppProducerCtx vctx cctx p1}, {ppProducerCtx vctx cctx p2}; {ppConsumerCtx vctx cctx c})"
+    | .ifz p s1 s2 =>
+        s!"ifz({ppProducerCtx vctx cctx p}, {ppStatementCtx vctx cctx s1}, {ppStatementCtx vctx cctx s2})"
+    | .cut p c => s!"⟨{ppProducerCtx vctx cctx p} | {ppConsumerCtx vctx cctx c}⟩"
 end
+
+def ppProducer (p : Producer) : String :=
+  ppProducerCtx [] [] p
+
+def ppConsumer (c : Consumer) : String :=
+  ppConsumerCtx [] [] c
+
+def ppStatement (s : Statement) : String :=
+  ppStatementCtx [] [] s
 
 instance : ToString Producer := ⟨ppProducer⟩
 instance : ToString Consumer := ⟨ppConsumer⟩
